define loop using power function and prove loop_fix

investigations/separate_loop_from_delay_in_timed_monad.v
@@ -1,4 +1,6 @@
 Require Import Coq.Lists.List. Import ListNotations.
+Require Import Coq.Arith.PeanoNat.
+Require Import Coq.micromega.Lia.
 
 (* based on https://github.com/project-oak/silveroak/blob/0adc80b5194a54afff21b7648dea4d3993dc2ea2/cava/Cava/Acorn/TimedMonad.v *)
 
@@ -30,12 +32,15 @@ Definition defaultCombValue(A: SignalType): combType A :=
   | Nat => 0
   end.
 
-Definition delay{A}(x: timed (combType A)): timed (combType A) :=
+Definition delayWithInit{A}(init: combType A)(x: timed (combType A)): timed (combType A) :=
   fun t =>
     match t with
-    | 0 => defaultCombValue A
+    | 0 => init
     | S t' => x t'
     end.
+
+Definition delay{A}(x: timed (combType A)): timed (combType A) :=
+  delayWithInit (defaultCombValue A) x.
 
 Definition incr(x: combType Nat): timed (combType Nat) :=
   ret (x + 1).
@@ -46,67 +51,10 @@ Definition decr(x: combType Nat): timed (combType Nat) :=
 Definition add(x y: combType Nat): timed (combType Nat) :=
   ret (x + y).
 
-Definition countUp: timed (combType Nat) := fun t => t.
-
 (* https://github.com/project-oak/silveroak/blob/0adc80b5194a54afff21b7648dea4d3993dc2ea2/cava/Cava/Acorn/SequentialTimed.v
 defines loopSeqF, which does a loop and a delay in the same construct.
 Can we define a construct that just adds the loop, but no delay?
 *)
-
-Module loop_bodies_with_cava_signatures.
-  Definition sample_loop_body_without_delay:
-    combType Nat * combType Nat -> timed (combType Nat) :=
-    fun '(inp, sum) =>
-      res <- add inp sum;;
-      res' <- incr res;;
-      res'' <- decr res';;
-      ret res''.
-
-  Definition sample_loop_body_with_delay:
-    combType Nat * combType Nat -> timed (combType Nat) :=
-    fun '(inp, sum) =>
-      res <- add inp sum;;
-      res' <- delay (incr res);;
-      res'' <- decr res';;
-      ret res''.
-
-  Definition loop {A B: SignalType}
-             (f: combType A * combType B -> timed (combType B))
-             (a: timed (combType A)): timed (combType B).
-    refine (fix rec(t: nat) :=
-              match t with
-              | 0 => defaultCombValue B
-              | S t_minus_one => _
-              end).
-    refine (f (a t, rec t) t).
-    Fail Defined. (* Recursive definition of rec is ill-formed. *)
-  Abort.
-
-  (* maybe delaying the termination checker until a concrete loop body
-     is known will help? *)
-  Notation "'loop' f" :=
-    (fun (a: timed (combType _)) =>
-       (fix rec(t: nat): combType _ :=
-          match t with
-          | 0 => defaultCombValue _
-          | S t_minus_one => f (a t, rec (S t_minus_one)) (S t_minus_one)
-          end))
-      (at level 10).
-
-  Fail Check (loop sample_loop_body_with_delay).
-  (* Nope: Recursive definition of rec is ill-formed. *)
-End loop_bodies_with_cava_signatures.
-
-(* let's try alternative signatures for the loop bodies *)
-Definition sample_loop_body_without_delay(inp_signal: timed (combType Nat)):
-  timed (combType Nat) -> timed (combType Nat) :=
-  fun sum_signal =>
-    inp <- inp_signal;;
-    sum <- sum_signal;;
-    res <- add inp sum;;
-    res' <- incr res;;
-    res'' <- decr res';;
-    ret res''.
 
 Definition sample_loop_body_with_delay(inp_signal: timed (combType Nat)):
   timed (combType Nat) -> timed (combType Nat) :=
@@ -118,39 +66,221 @@ Definition sample_loop_body_with_delay(inp_signal: timed (combType Nat)):
     res'' <- decr res';;
     ret res''.
 
-Definition loop {B: SignalType}
-           (f: timed (combType B) -> timed (combType B)): timed (combType B).
-  refine (fix rec(t: nat) :=
-            match t with
-            | 0 => defaultCombValue B
-            | S t_minus_one => _
-            end).
-  refine (f rec t).
-  Fail Defined. (* Recursive definition of rec is ill-formed. *)
-Abort.
+Definition power_fun{A: Type}(f: A -> A): nat -> A -> A :=
+  fix rec n :=
+    match n with
+    | O => id
+    | S n' => fun a => f (rec n' a)
+    end.
 
-(* maybe delaying the termination checker until a concrete loop body
-     is known will help? *)
-Notation "'loop' f" :=
-  (fix rec(t: nat): combType _ :=
-     match t with
-     | 0 => defaultCombValue _
-     | S t_minus_one => f rec (S t_minus_one)
-     end)
-  (at level 10).
+(* trick: if we want to know the value at time t, a fuel amount of (S t) is sufficient
+   (assuming that the loop body contains at least one delay), and we can completely
+   hide the fact that we use fuel inside the definition of loop *)
+Definition loop{B: SignalType}(f: timed (combType B) -> timed (combType B)): timed (combType B) :=
+  fun t => power_fun f (S t) (fun _ => defaultCombValue B) t.
 
+(* will be used with A, B, C instantiated to `timed Something` *)
+Definition compose{A B C}(f: A -> B)(g: B -> C): A -> C := fun a => g (f a).
+Infix ">>" := compose (at level 40).
+Definition fork2{A B}(f: A -> B): A -> B * B := fun a => let b := f a in (b, b).
+(* Take a pair input and apply the f to just the first element. *)
+Definition fsT{A1 A2 B}(f: A1 -> A2)(ab: A1 * B): A2 * B := let (a1, b) := ab in (f a1, b).
+(* Take a pair input and apply the f to just the second element. *)
+Definition snD{A B1 B2}(f: B1 -> B2)(ab: A * B1): A * B2 := let (a, b1) := ab in (a, f b1).
+
+Definition adder: timed (combType Nat) * timed (combType Nat) -> timed (combType Nat) :=
+  fun '(x, y) => v1 <- x;; v2 <- y;; add v1 v2.
+
+Eval cbv -[Nat.add] in adder.
+
+Definition const(A: SignalType)(v: combType A): combType A := v.
 
 Definition simulate{A: Type}(x: timed A)(n: nat): list A :=
   List.map x (List.seq 0 n).
 
+Definition incrementer(x: timed (combType Nat)): timed (combType Nat) :=
+  v <- x;; ret (v + 1).
+
+(*
+Here's a simple count up loop:
+
+      ---    -------
+      |i|    |delay|
+  +-->|n|--->|with |--+----->
+  |   |c|    |init |  |
+  |   |r|    |  0  |  |
+  |   ---    -------  |
+  |                   |
+  +-------------------+
+*)
+Definition countUp: timed (combType Nat) :=
+  loop (incrementer >> (delayWithInit (const Nat 0))).
+
+Compute simulate countUp 10. (* = [0; 1; 2; 3; 4; 5; 6; 7; 8; 9] *)
+
+(* We can pass this countUp loop as an input to another loop body: *)
 Definition sum_countUp: timed (combType Nat) :=
   loop (sample_loop_body_with_delay countUp).
-(* termination checker is happy because it unfolds `sample_loop_body_with_delay`
-   and `delay` and simplifies the term until it notices that the recursive
-   call is made with a structurally smaller nat *)
-
-Fail Definition sum_countUp_without_delay: timed (combType Nat) :=
-  loop (sample_loop_body_without_delay countUp).
-(* Recursive definition of rec is ill-formed. *)
 
 Compute simulate sum_countUp 10. (* = [0; 1; 3; 6; 10; 15; 21; 28; 36; 45] *)
+
+(*
+Here's a circuit with two delays computing Fibonacci numbers:
+
+      -------      -------   ---
+      |delay|      |delay|   | |
+  +-->|with |--+-->|with |-->|a|
+  |   |init |  |   |init |   |d|
+  |   |  1  |  |   |  0  |   |d|--+----->
+  |   -------  |   -------   |e|  |
+  |            |             |r|  |
+  |            +------------>| |  |
+  |                          ---  |
+  |                               |
+  +-------------------------------+
+
+*)
+Definition fib_body: timed (combType Nat) -> timed (combType Nat) :=
+  (fork2 (delayWithInit (const Nat 1)) >> fsT (delayWithInit (const Nat 0))) >> adder.
+Definition fib: timed (combType Nat) := loop fib_body.
+
+Compute simulate fib 10. (* = [1; 2; 3; 5; 8; 13; 21; 34; 55; 89] *)
+
+Definition equalUpTo{A}(t: nat)(x y: timed A) := forall u, u < t -> x u = y u.
+
+Lemma equalUpTo_elim{A}(x y: timed A):
+  (forall t, equalUpTo t x y) ->
+  forall t, x t = y t.
+Proof.
+  unfold equalUpTo.
+  intros E t.
+  apply (E (S t)).
+  constructor.
+Qed.
+
+Lemma equalUpTo_S{A}(x y: timed A)(t: nat):
+  equalUpTo t x y ->
+  x t = y t ->
+  equalUpTo (S t) x y.
+Proof.
+  unfold equalUpTo.
+  intros E1 E2 u L.
+  assert (u = t \/ u < t) as C by lia.
+  destruct C as [C | C].
+  - subst. exact E2.
+  - auto.
+Qed.
+
+Definition delaysAtLeast{A B}(f: timed A -> timed B)(d: nat) :=
+  forall a1 a2 t, equalUpTo t a1 a2 -> equalUpTo (t + d) (f a1) (f a2).
+
+Lemma power_fun_extra_fuel_has_no_effect{A}(f: timed (combType A) -> timed (combType A))(d: nat):
+  delaysAtLeast f (S d) ->
+  forall extra t u,
+  u < t ->
+  power_fun f (t + extra) (fun _ => defaultCombValue A) u =
+  power_fun f  t          (fun _ => defaultCombValue A) u.
+Proof.
+  induction t; intros.
+  - exfalso. lia.
+  - simpl.
+    unfold delaysAtLeast, equalUpTo in H.
+    eapply H with (t := u). 2: lia.
+    intros. eapply IHt. lia.
+Qed.
+
+Lemma loop_fix_aux{A}(f: timed (combType A) -> timed (combType A))(d: nat):
+  delaysAtLeast f (S d) ->
+  forall t, equalUpTo t (loop f) (f (loop f)).
+Proof.
+  unfold delaysAtLeast. intros D.
+  induction t.
+  - unfold equalUpTo.
+    intros ? C. inversion C.
+  - eapply equalUpTo_S. 1: exact IHt.
+    unfold loop at 1. simpl.
+    unfold loop.
+    unfold equalUpTo in D.
+    eapply D with (t := t). 2: lia.
+    intros.
+    replace t with (S u + (t - S u)) at 1 by lia.
+    rewrite (power_fun_extra_fuel_has_no_effect f d D) by lia.
+    reflexivity.
+Qed.
+
+Lemma loop_fix_without_funext{A}(f: timed (combType A) -> timed (combType A))(d: nat):
+  0 < d ->
+  delaysAtLeast f d ->
+  forall t, loop f t = f (loop f) t.
+Proof.
+  intros G D t.
+  eapply equalUpTo_elim.
+  destruct d. 1: inversion G.
+  eapply loop_fix_aux. exact D.
+Qed.
+
+Require Import Coq.Logic.FunctionalExtensionality.
+
+Lemma equalUpTo_eq{A}(x y: timed A):
+  (forall t, equalUpTo t x y) ->
+  x = y.
+Proof.
+  intro E.
+  extensionality t.
+  apply equalUpTo_elim.
+  exact E.
+Qed.
+
+(* If the loop body has a strictly positive delay, `loop` behaves like a fixpoint combinator: *)
+Theorem loop_fix{A}(f: timed (combType A) -> timed (combType A))(d: nat):
+  0 < d ->
+  delaysAtLeast f d ->
+  loop f = f (loop f).
+Proof.
+  intros G D. extensionality t. eapply loop_fix_without_funext; eassumption.
+Qed.
+
+Fixpoint fib_spec(n: nat): nat :=
+  match n with
+  | 0 => 1
+  | S n' => match n' with
+            | 0 => 2
+            | S n'' => fib_spec n'' + fib_spec n'
+            end
+  end.
+
+Goal simulate fib_spec 10 = simulate fib 10. compute. reflexivity. Qed.
+
+Lemma weaken_equalUpTo{A}(x y: timed A)(t1 t2: nat):
+  t1 <= t2 ->
+  equalUpTo t2 x y ->
+  equalUpTo t1 x y.
+Proof.
+  unfold equalUpTo. intros. eapply H0. lia.
+Qed.
+
+Lemma compose_delaysAtLeast{A B C}(f: timed A -> timed B)(g: timed B -> timed C)(d1 d2: nat):
+  delaysAtLeast f d1 ->
+  delaysAtLeast g d2 ->
+  delaysAtLeast (f >> g) (d1 + d2).
+Proof.
+  unfold compose, delaysAtLeast. intros. rewrite Nat.add_assoc. eauto.
+Qed.
+
+Lemma weaken_delaysAtLeast{A B}(f: timed A -> timed B)(d1 d2: nat):
+  delaysAtLeast f d2 ->
+  d1 <= d2 ->
+  delaysAtLeast f d1.
+Proof.
+  unfold delaysAtLeast. intros.
+  eapply weaken_equalUpTo. 2: eauto. lia.
+Qed.
+
+Lemma fib_body_delaysAtLeast: delaysAtLeast fib_body 1.
+Proof.
+  unfold fib_body.
+  eapply weaken_delaysAtLeast. {
+    match goal with
+    | |- delaysAtLeast (?f >> ?g) _ => eapply (compose_delaysAtLeast f g)
+    end.
+    (* requires changing signature of fork2 *)
